Fixing lift. Cleaning code.

IIO.Effect.fst
@@ -2,6 +2,7 @@ module IIO.Effect
 
 open FStar.Tactics
 open ExtraTactics
+open FStar.Calc
 
 open Common
 open IO.Free
@@ -9,25 +10,25 @@ open IO.Effect
 
 let rec iio_interpretation #a
   (m : iio a) 
-  (h : events_trace)
+  (h : trace)
   (p : io_post a) : Type0 = 
   match m with
   | Return x -> p (Inl x) []
   | Throw err -> p (Inr err) []
   | Cont (Call GetTrace args fnc) -> (
-      FStar.WellFounded.axiom1 fnc (Inl h);
-      iio_interpretation (fnc (Inl h)) h p
+    FStar.WellFounded.axiom1 fnc (Inl h);
+    iio_interpretation (fnc (Inl h)) h p
   )
   | Cont (Call cmd args fnc) -> (
     forall res. (
       FStar.WellFounded.axiom1 fnc res;
-      let event : io_event = convert_call_to_event cmd args res in
-      iio_interpretation (fnc res) (event::h) (gen_post p event)))
+      let e : event = convert_call_to_event cmd args res in
+      iio_interpretation (fnc res) (e::h) (gen_post p e)))
 
 
 // REFINED COMPUTATION MONAD (repr)
 let iio_irepr (a:Type) (wp:io_wpty a) =
-  h:events_trace -> post:io_post a ->
+  h:trace -> post:io_post a ->
     Pure (iio a)
       (requires (wp h post))
       (ensures (fun (t:iio a) -> iio_interpretation t h post))
@@ -35,14 +36,13 @@ let iio_irepr (a:Type) (wp:io_wpty a) =
 let iio_ireturn (a : Type) (x : a) : iio_irepr a (io_return_wp a x) =
   fun _ _ -> iio_return a x
 
-let w = io_wpty
-
-unfold
-val w_ord (#a : Type) : w a -> w a -> Type0
-let w_ord wp1 wp2 = forall h p. wp1 h p ==> wp2 h p
-
-let iio_ibind (a b : Type) (wp_v : w a) (wp_f: a -> w b) (v : iio_irepr a wp_v)
-  (f : (x:a -> iio_irepr b (wp_f x))) : iio_irepr b (io_bind_wp _ _ wp_v wp_f) =
+let iio_ibind 
+  (a b : Type) 
+  (wp_v : io_wpty a) 
+  (wp_f: a -> io_wpty b) 
+  (v : iio_irepr a wp_v)
+  (f : (x:a -> iio_irepr b (wp_f x))) : 
+  Tot (iio_irepr b (io_bind_wp _ _ wp_v wp_f)) =
   fun h p -> 
     let t = (iio_bind a b 
         (v h (compute_post a b h wp_f p))
@@ -53,15 +53,15 @@ let iio_ibind (a b : Type) (wp_v : w a) (wp_f: a -> w b) (v : iio_irepr a wp_v)
     t
 
 unfold
-let isubcomp (a:Type) (wp1 wp2: w a) (f : iio_irepr a wp1) :
-  Pure (iio_irepr a wp2) (requires w_ord wp2 wp1) (ensures fun _ -> True) = f
+let isubcomp (a:Type) (wp1 wp2: io_wpty a) (f : iio_irepr a wp1) :
+  Pure (iio_irepr a wp2) (requires io_wpty_ord wp2 wp1) (ensures fun _ -> True) = f
 
 unfold
-let wp_if_then_else (#a:Type) (wp1 wp2:w a) (b:bool) : w a =
+let wp_if_then_else (#a:Type) (wp1 wp2:io_wpty a) (b:bool) : io_wpty a =
   fun h p -> (b ==> wp1 h p) /\ ((~b) ==> wp2 h p)
 
 unfold
-let i_if_then_else (a : Type) (wp1 wp2 : w a) (f : iio_irepr a wp1) (g : iio_irepr a wp2) (b : bool) : Type =
+let i_if_then_else (a : Type) (wp1 wp2 : io_wpty a) (f : iio_irepr a wp1) (g : iio_irepr a wp2) (b : bool) : Type =
   iio_irepr a (wp_if_then_else wp1 wp2 b)
 
 total
@@ -85,50 +85,82 @@ let lift_pure_iiowp (a:Type) (wp:pure_wp a) (f:(eqtype_as_type unit -> PURE a wp
 
 sub_effect PURE ~> IOwp = lift_pure_iowp
 
-// let rec cast_io_iio #a (x:io a) : iio a =
-//   match x with
-//   | Return z -> Return z
-//   | Throw z -> Throw z
-//   | Cont (Call cmd args fnc) ->
-//          Cont (Call cmd args (fun res ->
-//            FStar.WellFounded.axiom1 fnc res;
-//            cast_io_iio (fnc res)))
+let rec cast_io_iio #a (x:io a) : iio a =
+  match x with
+  | Return z -> Return z
+  | Throw z -> Throw z
+  | Cont (Call (cmd:io_cmds) args fnc) ->
+     Cont (Call cmd args (fun res ->
+       FStar.WellFounded.axiom1 fnc res;
+       cast_io_iio (fnc res)))
+
+let rec io_interp_to_iio_interp' (#a:Type u#a) 
+  (cmd:io_cmds) (arg:io_args cmd) (fnc:(io_resm cmd -> sys io_cmds io_sig a)) 
+  (h:trace) (p:io_post a) 
+  (r:(io_resm cmd)) :
+  Lemma
+    (requires 
+      (io_interpretation 
+        (fnc r) 
+        (gen_post p (convert_call_to_event cmd arg r))))
+    (ensures (
+      let e : event = convert_call_to_event cmd arg r in
+      iio_interpretation 
+        (cast_io_iio (fnc r)) 
+        (e::h) 
+        (gen_post p e))) 
+    (decreases fnc) =
+  let e : event = convert_call_to_event cmd arg r in
+  FStar.WellFounded.axiom1 fnc r;
+  match fnc r with
+  | Cont (Call cmd' arg' fnc') ->
+      Classical.forall_intro (Classical.move_requires (io_interp_to_iio_interp' cmd' arg' fnc' (e::h) (gen_post p e)))
+  | _ -> ()
+
+let io_interp_to_iio_interp (#a:Type u#a) (x:io a) (h:trace) (p:io_post a) : 
+  Lemma
+    (requires (io_interpretation x p))
+    (ensures  (iio_interpretation (cast_io_iio x) h p)) =
+  match x with
+  | Cont (Call (cmd:io_cmds) arg fnc) -> 
+      Classical.forall_intro (Classical.move_requires (io_interp_to_iio_interp' cmd arg fnc h p))
+  | _ -> ()
 
 let lift_iowp_iiowp (a:Type) (wp:io_wpty a) (f:io_irepr a wp) :
   Pure (iio_irepr a (fun s0 p -> wp s0 (fun r le -> p r le))) 
     (requires True)
-    (ensures (fun _ -> True))
-  // TODO: lift from IO.irepr to IIO.iio_irepr
-  = fun s0 p -> admit (); f s0 p
+    (ensures (fun _ -> True)) = 
+  fun s0 p ->
+    io_interp_to_iio_interp (f s0 p) s0 p;
+    cast_io_iio (f s0 p)
 
 sub_effect IOwp ~> IIOwp = lift_iowp_iiowp
   
-effect IIOi
+effect IIOPrePost
   (a:Type)
-  (pre : events_trace -> Type0)
-  (post : events_trace -> maybe a -> events_trace -> Type0) =
-  IIOwp a (fun (h:events_trace) (p:io_post a) ->
+  (pre : trace -> Type0)
+  (post : trace -> maybe a -> trace -> Type0) =
+  IIOwp a (fun (h:trace) (p:io_post a) ->
     pre h /\ (forall res le. post h res le ==>  p res le))
 
-let get_trace () : IIOi events_trace (fun h -> True) 
-  (fun h r le -> r == (Inl h) /\ le == []) =
+let get_trace () : IIOwp trace 
+  (fun h p -> forall r le. r == (Inl h) /\ le == [] ==>  p r le) =
   IIOwp?.reflect (fun _ _ -> sys_perform (Call GetTrace () (fun h -> h)))
 
-let throw (err:exn) : IIOwp events_trace (fun _ p -> p (Inr err) []) =
+let throw (err:exn) : IIOwp trace (fun _ p -> p (Inr err) []) =
   IIOwp?.reflect(fun _ _ -> iio_throw _ err)
 
 let pi_static_cmd
   (cmd : io_cmds)
   (pi : monitorable_prop)
   (arg : args cmd) :
-  IIOi (res cmd)
+  IIOPrePost (res cmd)
     (requires (fun h ->
       default_check h (| cmd, arg |) &&
       pi h (| cmd, arg |)))
     (ensures (fun h r le ->
       (match r with
-      | Inr GIO_pi_failed -> False
-      | Inr GIO_default_check_failed -> False
+      | Inr Contract_failure -> False
       | _ -> le == [convert_call_to_event cmd arg r])
       /\ enforced_locally default_check h le
       /\ enforced_locally pi h le)) =
@@ -138,12 +170,11 @@ let mixed_cmd
   (cmd : io_cmds)
   (pi : monitorable_prop)
   (arg : args cmd) :
-  IIOi (res cmd)
+  IIOPrePost (res cmd)
     (requires (fun s0 -> default_check s0 (| cmd, arg |)))
     (ensures (fun h r le ->
       (match r with
-      | Inr GIO_default_check_failed -> False
-      | Inr GIO_pi_failed -> le == []
+      | Inr Contract_failure -> le == []
       | _ -> le == [convert_call_to_event cmd arg r])
       /\ enforced_locally default_check h le
       /\ enforced_locally pi h le
@@ -152,18 +183,17 @@ let mixed_cmd
   let action = (| cmd, arg |) in
   match pi s0 action with
   | true -> pi_static_cmd cmd pi arg
-  | false -> throw GIO_pi_failed
+  | false -> throw Contract_failure 
 
 let dynamic_cmd
   (cmd : io_cmds)
   (pi : monitorable_prop)
   (arg : args cmd) :
-  IIOi (res cmd) 
+  IIOPrePost (res cmd) 
     (requires (fun s0 -> True))
     (ensures (fun h r le ->
       (match r with
-      | Inr GIO_default_check_failed
-      | Inr GIO_pi_failed -> le == []
+      | Inr Contract_failure -> le == []
       | _ -> le == [convert_call_to_event cmd arg r])
       /\ enforced_locally default_check h le
       /\ enforced_locally pi h le
@@ -172,26 +202,26 @@ let dynamic_cmd
   let action = (| cmd, arg |) in
   match default_check s0 action with
   | true -> mixed_cmd cmd pi arg
-  | false -> throw GIO_default_check_failed
+  | false -> throw Contract_failure
 
-let iio_pre (pi_check : monitorable_prop) (s0:events_trace) : Type0 =
+let iio_pre (pi : monitorable_prop) (s0:trace) : Type0 =
   enforced_globally default_check s0 &&
-  enforced_globally pi_check s0
+  enforced_globally pi s0
 
-let iio_invariant_post
+let iio_post
   (#a:Type)
-  (pi_check : monitorable_prop)
-  (s0:events_trace)
+  (pi : monitorable_prop)
+  (s0:trace)
   (result:maybe a)
-  (local_trace:events_trace) :
+  (local_trace:trace) :
   Tot Type0 =
   enforced_globally (default_check) (apply_changes s0 local_trace) /\
-  enforced_globally (pi_check) (apply_changes s0 local_trace)
+  enforced_globally (pi) (apply_changes s0 local_trace)
 
 effect IIO 
   (a:Type)
-  (pi_check : monitorable_prop) 
-  (post : events_trace -> maybe a -> events_trace -> Type0) =
-  IIOi a
-    (requires (iio_pre pi_check))
-    (ensures (fun h r le -> iio_invariant_post pi_check h r le /\ post h r le))
+  (pi : monitorable_prop) 
+  (post : trace -> maybe a -> trace -> Type0) =
+  IIOPrePost a
+    (requires (iio_pre pi))
+    (ensures (fun h r le -> iio_post pi h r le /\ post h r le))
