IO.Effect.fst
@@ -6,38 +6,32 @@ open ExtraTactics
 open Common
 open IO.Free
 
-let io_post a = maybe a -> events_trace -> Type0  // local_events (from old to new)
-let io_wpty a = events_trace -> io_post a -> Type0  // past_events (from new to old; reversed compared with local_events)
+let io_post a = maybe a -> trace -> Type0  // local_events (from old to new)
+let io_wpty a = trace -> io_post a -> Type0  // past_events (from new to old; reversed compared with local_events)
 
 unfold
 let io_return_wp (a:Type) (x:a) : io_wpty a =
-  fun past_events p -> p (Inl x) []
+  fun _ p -> p (Inl x) []
 
 unfold
-let compute_post (a b:Type) (past_events:events_trace) (kw : a -> io_wpty b) (p:io_post b)
+let compute_post (a b:Type) (h:trace) (kw : a -> io_wpty b) (p:io_post b)
   : io_post a =
       (fun result local_events -> 
         match result with
         | Inl result -> (
             kw result
-            ((List.rev local_events) @ past_events) 
+            ((List.rev local_events) @ h) 
             (fun result' local_events' -> 
                 p result' (local_events @ local_events')))
         | Inr err -> p (Inr err) local_events)
 
 unfold
 let io_bind_wp (a:Type) (b:Type) (w : io_wpty a) (kw : a -> io_wpty b) : io_wpty b =
-  fun past_events p -> 
-    w past_events (compute_post a b past_events kw p)
+  fun h p -> 
+    w h (compute_post a b h kw p)
 
-unfold let gen_post #a (post:io_post a) (event:io_event) = 
-  fun x local_events -> post x (event :: local_events)
-
-unfold let convert_call_to_event (cmd:io_cmds) (args:args cmd) (res:resm cmd) =
-  match cmd with
-  | Openfile -> EOpenfile args res
-  | Read -> ERead args res
-  | Close -> EClose args res
+let gen_post #a (post:io_post a) (e:event) = 
+  fun x local_events -> post x (e :: local_events)
 
 // It is weird that this interpretation knows about
 // contract failure. Somebody will be able to throw this errors
@@ -51,15 +45,15 @@ let rec io_interpretation #a
   | Return x -> p (Inl x) []
   | Throw err -> p (Inr err) []
   | Cont (Call cmd args fnc) -> (
-    forall res. (Inr? res ==>  ~(Inr?.v res == GIO_pi_failed \/ Inr?.v res == GIO_default_check_failed)) ==> (
+    forall res. (
       FStar.WellFounded.axiom1 fnc res;
-      let event : io_event = convert_call_to_event cmd args res in
-      io_interpretation (fnc res) (gen_post p event)))
+      let e : event = convert_call_to_event cmd args res in
+      io_interpretation (fnc res) (gen_post p e)))
 
 
 // REFINED COMPUTATION MONAD (repr)
 let io_irepr (a:Type) (wp:io_wpty a) =
-  h:events_trace -> post:io_post a ->
+  h:trace -> post:io_post a ->
     Pure (io a)
       (requires (wp h post))
       (ensures (fun (t:io a) -> io_interpretation t post))
@@ -67,17 +61,11 @@ let io_irepr (a:Type) (wp:io_wpty a) =
 let io_ireturn (a : Type) (x : a) : io_irepr a (io_return_wp a x) =
   fun _ _ -> io_return a x
 
-let w = io_wpty
-
 unfold
-val w_ord (#a : Type) : w a -> w a -> Type0
-let w_ord wp1 wp2 = forall h p. wp1 h p ==> wp2 h p
+val io_wpty_ord (#a : Type) : io_wpty a -> io_wpty a -> Type0
+let io_wpty_ord wp1 wp2 = forall h p. wp1 h p ==> wp2 h p
 
-unfold
-let apply_changes (old_state local_trace:events_trace) = (List.rev local_trace) @ old_state
-
-
-let io_ibind (a b : Type) (wp_v : w a) (wp_f: a -> w b) (v : io_irepr a wp_v)
+let io_ibind (a b : Type) (wp_v : io_wpty a) (wp_f: a -> io_wpty b) (v : io_irepr a wp_v)
   (f : (x:a -> io_irepr b (wp_f x))) : io_irepr b (io_bind_wp _ _ wp_v wp_f) =
   fun h p -> 
     let t = (io_bind a b 
@@ -89,15 +77,15 @@ let io_ibind (a b : Type) (wp_v : w a) (wp_f: a -> w b) (v : io_irepr a wp_v)
     t
 
 unfold
-let isubcomp (a:Type) (wp1 wp2: w a) (f : io_irepr a wp1) :
-  Pure (io_irepr a wp2) (requires w_ord wp2 wp1) (ensures fun _ -> True) = f
+let isubcomp (a:Type) (wp1 wp2: io_wpty a) (f : io_irepr a wp1) :
+  Pure (io_irepr a wp2) (requires io_wpty_ord wp2 wp1) (ensures fun _ -> True) = f
 
 unfold
-let wp_if_then_else (#a:Type) (wp1 wp2:w a) (b:bool) : w a =
+let wp_if_then_else (#a:Type) (wp1 wp2:io_wpty a) (b:bool) : io_wpty a =
   fun h p -> (b ==> wp1 h p) /\ ((~b) ==> wp2 h p)
 
 unfold
-let i_if_then_else (a : Type) (wp1 wp2 : w a) (f : io_irepr a wp1) (g : io_irepr a wp2) (b : bool) : Type =
+let i_if_then_else (a : Type) (wp1 wp2: io_wpty a) (f : io_irepr a wp1) (g : io_irepr a wp2) (b : bool) : Type =
   io_irepr a (wp_if_then_else wp1 wp2 b)
 
 total
@@ -123,14 +111,14 @@ sub_effect PURE ~> IOwp = lift_pure_iowp
   
 effect IO
   (a:Type)
-  (pre : events_trace -> Type0)
-  (post : events_trace -> maybe a -> events_trace -> Type0) =
-  IOwp a (fun (h:events_trace) (p:io_post a) ->
+  (pre : trace -> Type0)
+  (post : trace -> maybe a -> trace -> Type0) =
+  IOwp a (fun (h:trace) (p:io_post a) ->
     pre h /\ (forall res le. post h res le ==>  p res le))
 
-let rec is_open (fd:file_descr) (past_events: events_trace) :
+let rec is_open (fd:file_descr) (h: trace) :
   Tot bool =
-  match past_events with
+  match h with
   | [] -> false
   | h :: tail -> match h with
                | EOpenfile _ (Inl fd') ->
@@ -142,11 +130,11 @@ let rec is_open (fd:file_descr) (past_events: events_trace) :
                | _ -> is_open fd tail
 
 val default_check : monitorable_prop
-let default_check (state:events_trace) (action:action_type) =
+let default_check (h:trace) (action:action_type) =
   match action with
   | (| Openfile, fnm |) -> true
-  | (| Read, fd |) -> is_open fd state
-  | (| Close, fd |) -> is_open fd state
+  | (| Read, fd |) -> is_open fd h
+  | (| Close, fd |) -> is_open fd h
 
 let static_cmd
   (cmd : io_cmds)
@@ -155,10 +143,9 @@ let static_cmd
     (requires (fun h -> default_check h (| cmd, argz |)))
     (ensures (fun h r local_trace ->
       (match r with
-      | Inr GIO_pi_failed -> False
-      | Inr GIO_default_check_failed -> False
+      | Inr Contract_failure -> False
       | _ -> True) /\
       local_trace == [convert_call_to_event cmd argz r]
       /\ enforced_locally default_check h local_trace
-  )) by (compute ()) =
-  IOwp?.reflect(fun _ _ -> io_all cmd argz)
+  )) =
+  IOwp?.reflect(fun _ _ -> io_call cmd argz)
